P(x) = W(x) \* Q(x) + R(x)
- P(x) is the top on divide
- Q(x) is the bottom on divide
- W(x) / I(x) is the result
- R(x) is the remainder

Wielomian stopnia 3 pierwiastki
x2 = Sprezenie x1 (if is z)
x3 = (x - x1)(x - x2) -> Long divide result by P(x) which gives you (x + a) and x<sub>3</sub> = -a

Wielomian stopnia 4 pierwiastki
x2 = Sprezenie x1
x3, x4 = (x - x1)(x - x2) -> W(x):result which gives you (x<sup>2</sup> + a) and x<sub>3</sub> = a, x<sub>4</sub> = -a

Wielomian stopnia 6 pierwiastki
x1, x2 = given
x3, x4 = Sprezenie x1, x2
x5, x6 = 
- (x - x1)(x - x3)(x - x2)(x - x4) // Can multiply normal * sprezenie for each then multiply both
- Result of W(x):above, results in R(x) and Q(x), Q(x) = 0 is result

Important for finding pierwiastki when long div remainder needs to be 0 or you fucked up
sqrt(-4) = 2i
sqrt(-16) = 4i
sqrt(-2) = sqrt(2) \* i

Przedstaw w postaci iloczynu dwuminaow (pytanie ktore ma z I znajdujesz delta)
Remember to label as z<sub>1</sub> 

For z<sup>3</sup> You can guess z<sub>1</sub> by finding which values equation is 0 for then divide main equation by z - z<sub>1</sub>  and solving that

Zad 4 Wielomian rzecywiste (High power), know these formulas and reshape, remember they have to be real numbers

a<sup>3</sup> + b<sup>3</sup> = (a + b)(a<sup>2</sup> - ab + b<sup>2</sup>)
a<sup>3</sup> - b<sup>3</sup> = (a - b)(a<sup>2</sup> + ab + b<sup>2</sup>)

a<sup>2</sup> + b<sup>2</sup> = (a + bi)(a - bi)
a<sup>2</sup> - b<sup>2</sup> = (a - b)(a + b)
(a + b)<sup>2</sup> = a<sup>2</sup> + 2ab + b<sup>2</sup>
(a - b)<sup>2</sup> = a<sup>2</sup> - 2ab + b<sup>2</sup>

z<sup>2</sup> + 4 = z<sup>2</sup> - (-4) = (z + 2i)(z - 2i) because sqrt(-4) = 2i

Also remember that you can display imaginary numbers as real by doing (x<sup>2</sup> - (1 - i))(x<sup>2</sup> - (1 + i)) then multiplying out

Rozlozyc na ulamki proste
- z^2 = (z - 1)(z + 2)
- z^2 = A / (z - 1) + B / (z + 2)
- z^2 = A(z + 2) + B(z - 1)
- Now you cover up or all parts by power
- For (z + 2)^2 remember you have to do A(z + 2) then B(z + 2)^2
- For (z^2 + 2) remember you have to do Ax + B (or Az + B)